pulse/test/nolib/Match.fst
@@ -1,0 +1,59 @@
+module Match
+
+#lang-pulse
+open Pulse.Nolib
+
+type t1 = | A | B
+type t2 =
+  | C : x:int -> y:int{x > y} -> t2
+  | D
+
+assume val foo : int -> slprop
+
+let rel (x: t1) (y: t2) : slprop =
+  match x, y with
+  | A, C _ _ -> foo 1
+  | B, D -> foo 2
+  | _ -> pure False
+
+let rel_cases_pred (x:t1) (y:t2) : bool =
+  match x, y with
+  | A, C _ _ -> true
+  | B, D -> true
+  | _ -> false
+
+ghost
+fn rel_cases (x:t1) (y:t2)
+  requires rel x y
+  ensures  rel x y ** pure (rel_cases_pred x y)
+{
+  if (rel_cases_pred x y) {
+    ()
+  } else {
+    rewrite rel x y as pure False;
+    unreachable ();
+  }
+}
+
+fn test (x : t1) (y z : t2)
+  requires rel x y ** rel x z
+  ensures rel x y ** rel x z ** pure (C? y == C? z)
+{
+  rel_cases x y;
+  rel_cases x z;
+  match x {
+    A -> {
+      let C y1 y2 = y;
+      let C z1 z2 = z;
+      rewrite each C z1 z2 as z;
+      rewrite each C y1 y2 as y;
+      rewrite each A as x;
+      ()
+    }
+    B -> {
+      let D = y;
+      let D = z;
+      ();
+    }
+  }
+}
